test/lint_simp_nonconfl.lean
@@ -1,0 +1,18 @@
+import tactic.lint
+
+def f : ℕ → ℕ := default _
+def g : ℕ → ℕ := default _
+def c : ℕ := default _
+def d : ℕ := default _
+
+-- The following TRS is non-confluent, since `f d <-- f (g c) --> c` is not joinable
+@[simp] lemma a : g c = d := rfl
+@[simp] lemma b {x} : f (g x) = c := rfl
+
+open tactic
+#eval do
+decl ← get_decl ``b,
+res ← linter.simp_nonconfl.test decl,
+-- linter complains
+trace res,
+guard $ res.is_some
